packages/zoe/spec/ocpl/modern_heap.v
@@ -1,0 +1,142 @@
+(* Modernized OCPL-style low-integrity layer for current Iris HeapLang. *)
+From stdpp Require Import gmap.
+From iris.algebra Require Import ofe.
+From iris.bi.lib Require Import fixpoint_banach.
+From iris.proofmode Require Import proofmode.
+From iris.program_logic Require Export weakestpre.
+From iris.heap_lang Require Export lang metatheory primitive_laws.
+From iris.heap_lang Require Import notation proofmode.
+
+Module OCPLModernHeap.
+  Open Scope expr_scope.
+
+  Definition env := gmap string val.
+
+  Class LowIntegrity Σ (A : Type) := Low {
+    low : A -> iProp Σ;
+    #[global] low_persistent a :: Persistent (low a);
+    #[global] low_ne n :: Proper ((=) ==> dist n) low
+  }.
+  Arguments Low {_ _} _ _ _.
+  Arguments low {_ _ _} _ : simpl never.
+  Instance : Params (@low) 3 := {}.
+
+  Global Instance low_proper `{LowIntegrity Σ A} :
+    Proper ((=) ==> (≡)) low.
+  Proof. solve_proper. Qed.
+
+  Section low_values.
+    Context {Σ : gFunctors}.
+    Context {hlc : has_lc}.
+    Context `{!heapGS_gen hlc Σ}.
+    Context `{!LowIntegrity Σ loc}.
+
+    Definition low_pre (self : val -d> iPropO Σ) : val -d> iPropO Σ :=
+      OfeMor (λ v,
+        match v with
+        | LitV (LitLoc l) => low l
+        | LitV _ => True
+        | RecV f x e =>
+            □ ▷ ∀ w, self w -∗
+              WP (subst' x w (subst' f (RecV f x e) e)) @ NotStuck; ⊤
+                {{ v', self v' }}
+        | PairV v1 v2 => ▷ (self v1 ∗ self v2)
+        | InjLV v | InjRV v => ▷ self v
+        end)%I.
+
+    Global Instance low_pre_contractive :
+      Contractive low_pre.
+    Proof. solve_contractive. Qed.
+
+    Definition low_val : val -d> iPropO Σ := fixpoint low_pre.
+
+    Global Instance low_val_persistent v : Persistent (low_val v).
+    Proof.
+      apply (fixpoint_persistent low_pre).
+      intros Φ HΦ w.
+      destruct w as [l|f x e|v1 v2|vinl|vinr]; simpl.
+      - destruct l; simpl; apply _.
+      - apply _.
+      - apply _.
+      - apply _.
+      - apply _.
+    Qed.
+
+    Global Instance val_low : LowIntegrity Σ val :=
+      Low low_val _ _.
+
+    Lemma low_loc l :
+      low l ⊣⊢ low (A := loc) l.
+    Proof. done. Qed.
+
+    Lemma low_val_eq v :
+      low v ⊣⊢ low_val v.
+    Proof. done. Qed.
+
+    Lemma low_val_unfold v :
+      low v ⊣⊢
+      match v with
+        | LitV (LitLoc l) => low (A := loc) l
+        | LitV _ => True
+        | RecV f x e =>
+          □ ▷ ∀ w, low_val w -∗
+            WP (subst' x w (subst' f (RecV f x e) e)) @ NotStuck; ⊤
+              {{ v', low_val v' }}
+      | PairV v1 v2 => ▷ (low_val v1 ∗ low_val v2)
+      | InjLV v | InjRV v => ▷ low_val v
+      end.
+    Proof.
+      rewrite low_val_eq.
+      change (low_val v ⊣⊢ low_pre low_val v).
+      rewrite /low_val.
+      apply (fixpoint_unfold low_pre v).
+    Qed.
+
+    Global Instance env_low : LowIntegrity Σ env :=
+      Low (λ γ, [∗ map] v ∈ γ, low v)%I _ _.
+
+    Lemma low_env γ :
+      low γ ⊣⊢ [∗ map] v ∈ γ, low v.
+    Proof. done. Qed.
+
+    Lemma low_env_empty :
+      low (∅ : env) ⊣⊢ True.
+    Proof. exact: big_sepM_empty. Qed.
+
+    Lemma low_env_insert γ x v :
+      γ !! x = None ->
+      low v -∗ low γ -∗ low (<[x := v]> γ).
+    Proof.
+      iIntros (?) "#Hv #Hγ".
+      rewrite !low_env.
+      iApply (big_sepM_insert_2 (λ _ w, low w)%I with "Hv").
+      iExact "Hγ".
+    Qed.
+
+    Lemma low_env_singleton x v :
+      low ({[x := v]} : env) ⊣⊢ low v.
+    Proof. exact: big_sepM_singleton. Qed.
+
+    Lemma low_env_lookup γ x v :
+      γ !! x = Some v ->
+      low γ -∗ low v.
+    Proof.
+      iIntros (?) "Hγ".
+      rewrite low_env.
+      iDestruct (big_sepM_lookup (λ _ w, low w)%I γ x v with "Hγ") as "$"; done.
+    Qed.
+
+    Lemma low_env_delete γ x :
+      low γ -∗ low (delete x γ).
+    Proof.
+      iIntros "Hγ".
+      rewrite !low_env.
+      destruct (γ !! x) as [v|] eqn:Hlookup.
+      - rewrite (big_sepM_delete (λ _ w, low w)%I γ x v); [|done].
+        iDestruct "Hγ" as "[_ Hγ]".
+        iExact "Hγ".
+      - rewrite delete_notin; [done|].
+        done.
+    Qed.
+  End low_values.
+End OCPLModernHeap.
